compiler/dsl/coq/ReflexDenoted.v
@@ -1,0 +1,15 @@
+Class Denoted (T : Type) : Type :=
+{ denote : T -> Type
+}.
+Notation "[[ x ]]" := (denote x).
+
+Definition optdenote {T} `{Denoted T} (ox : option T) :=
+  match ox with
+  | None => False
+  | Some x => [[ x ]]
+  end.
+Notation "[! x !]" := (optdenote x).
+
+Instance Denoted_option {T} `{ Denoted T } : Denoted (option T) :=
+{ denote := optdenote
+}.
