compiler/dsl/coq/ReflexFin.v
@@ -1,0 +1,5 @@
+Fixpoint fin (n : nat) : Type :=
+  match n with
+  | O => False
+  | S n' => option (fin n')
+  end.
