compiler/dsl/coq/ReflexHVec.v
@@ -1,0 +1,37 @@
+Require Import ReflexDenoted.
+Require Import ReflexFin.
+Require Import ReflexVec.
+
+Section HeterogeneousVector.
+
+Variable desc : Type.
+Variable Instance denote_desc : Denoted desc.
+
+Fixpoint hvec (n : nat) : vec desc n -> Type :=
+  match n with
+  | O => fun _ => unit
+  | S n' => fun v =>
+    match v with
+    | (t, v') => [[ t ]] * hvec n' v'
+    end
+  end%type.
+
+Fixpoint hv_nth (n : nat) (v_d : vec desc n) (v : hvec n v_d) (i : fin n)
+  : [[ v_get desc n v_d i ]] :=
+  match n as _n return
+    forall (v_d : vec desc _n) (v : hvec _n v_d) (i : fin _n), [[ v_get desc _n v_d i ]]
+  with
+  | O => fun v_d v i => match i with end
+  | S n' => fun (v_d : desc * vec desc n') (v : hvec (S n') v_d) i =>
+    match v_d as _v_d return
+      forall (v : hvec (S n') _v_d) (i : fin (S n')), [[ v_get desc (S n') _v_d i ]]
+    with
+    | (t, v_d') => fun (v : [[ t ]] * hvec n' v_d') (i : fin (S n')) =>
+      match i with
+      | None => fst v
+      | Some i' => hv_nth n' v_d' (snd v) i'
+      end
+    end v i
+  end v_d v i.
+
+End HeterogeneousVector.
