compiler/dsl/coq/ReflexVec.v
@@ -1,0 +1,23 @@
+Require Import ReflexFin.
+
+Section Vector.
+
+Variable T : Type.
+
+Fixpoint vec (n : nat) : Type :=
+  match n with
+  | O => unit
+  | S n' => T * vec n'
+  end%type.
+
+Fixpoint v_get (n : nat) : vec n -> fin n -> T :=
+  match n with
+  | O => fun _ idx => match idx with end
+  | S n' => fun v idx =>
+    match idx with
+    | None => fst v
+    | Some idx' => v_get n' (snd v) idx'
+    end
+  end.
+
+End Vector.
